theories/proofmode/solve_addr.v
@@ -10,114 +10,229 @@ Tactic Notation "solve_addr" "+" hyp_list(Hs) := clear -Hs; solve_addr.
 
 (* --------------------------- BASIC LEMMAS --------------------------------- *)
 
-(** Address arithmetic *)
+(** Physical Address arithmetic *)
 
-Lemma addr_add_0 a: (a + 0)%a = Some a.
+Lemma phys_addr_add_0 (a: PhysAddr): (a + 0)%a = Some a.
 Proof. solve_addr. Qed.
 
-Lemma incr_addr_one_none a :
+Lemma incr_phys_addr_one_none (a: PhysAddr) :
   (a + 1)%a = None ->
-  a = top.
+  a = top_phys.
 Proof. solve_addr. Qed.
 
-Lemma incr_addr_opt_add_twice (a: Addr) (n m: Z) :
+Lemma incr_phys_addr_opt_add_twice (a: PhysAddr) (n m: Z) :
   (0 <= n)%Z ->
   (0 <= m)%Z ->
   ((a ^+ n) ^+ m)%a = (a ^+ (n + m)%Z)%a.
 Proof. solve_addr. Qed.
 
-Lemma incr_addr_opt_add_twice' (a: Addr) (n m: Z) :
+Lemma incr_phys_addr_opt_add_twice' (a: PhysAddr) (n m: Z) :
   (0 <= n)%Z ->
   (0 <= m)%Z ->
   ((a ^+ n) ^+ m)%a = (a ^+ (n + m)%Z)%a.
 Proof. zify_addr;[]. (* only one goal! *) lia. Qed.
 
-Lemma top_le_eq a : (top <= a)%a → a = top.
+Lemma phys_top_le_eq (a: PhysAddr) : (top_phys <= a)%a → a = top_phys.
 Proof. solve_addr. Qed.
 
-Lemma top_not_le_eq a : ¬ (a < top)%a → a = top.
+Lemma phys_top_not_le_eq (a: PhysAddr) : ¬ (a < top_phys)%a → a = top_phys.
 Proof. solve_addr. Qed.
 
-Lemma next_lt (a a' : Addr) :
+Lemma phys_next_lt (a a' : PhysAddr) :
   (a + 1)%a = Some a' → (a < a')%Z.
 Proof. solve_addr. Qed.
 
-Lemma next_lt_i (a a' : Addr) (i : Z) :
+Lemma phys_next_lt_i (a a' : PhysAddr) (i : Z) :
   (i > 0)%Z →
   (a + i)%a = Some a' → (a < a')%Z.
 Proof. solve_addr. Qed.
 
-Lemma next_le_i (a a' : Addr) (i : Z) :
+Lemma phys_next_le_i (a a' : PhysAddr) (i : Z) :
   (i >= 0)%Z →
   (a + i)%a = Some a' → (a <= a')%Z.
 Proof. solve_addr. Qed.
 
-Lemma next_lt_top (a : Addr) i :
+Lemma phys_next_lt_top (a : PhysAddr) i :
   (i > 0)%Z →
-  is_Some (a + i)%a → a ≠ top.
+  is_Some (a + i)%a → a ≠ top_phys.
 Proof. intros ? [? ?] ?. solve_addr. Qed.
 
-Lemma addr_next_le (a e : Addr) :
+Lemma phys_addr_next_le (a e : PhysAddr) :
   (a < e)%Z → ∃ a', (a + 1)%a = Some a'.
 Proof. intros. zify_addr; eauto. exfalso. lia. lia. Qed.
 
-Lemma addr_next_lt (a e : Addr) :
+Lemma phys_addr_next_lt (a e : PhysAddr) :
   (a < e)%Z -> ∃ a', (a + 1)%a = Some a'.
 Proof. intros. zify_addr; eauto. exfalso. lia. lia. Qed.
 
-Lemma addr_next_lt_gt_contr (a e a' : Addr) :
+Lemma phys_addr_next_lt_gt_contr (a e a' : PhysAddr) :
   (a < e)%Z → (a + 1)%a = Some a' → (e < a')%Z → False.
 Proof. solve_addr. Qed.
 
-Lemma addr_next_lt_le (a e a' : Addr) :
+Lemma phys_addr_next_lt_le (a e a' : PhysAddr) :
   (a < e)%Z → (a + 1)%a = Some a' → (a' ≤ e)%Z.
 Proof. solve_addr. Qed.
 
-Lemma addr_abs_next (a e a' : Addr) :
+Lemma phys_addr_abs_next (a e a' : PhysAddr) :
   (a + 1)%a = Some a' → (a < e)%Z → (Z.abs_nat (e - a) - 1) = (Z.abs_nat (e - a')).
 Proof. solve_addr. Qed.
 
-Lemma incr_addr_trans (a1 a2 a3 : Addr) (z1 z2 : Z) :
+Lemma incr_phys_addr_trans (a1 a2 a3 : PhysAddr) (z1 z2 : Z) :
   (a1 + z1)%a = Some a2 → (a2 + z2)%a = Some a3 →
   (a1 + (z1 + z2))%a = Some a3.
 Proof. solve_addr. Qed.
 
-Lemma addr_add_assoc (a a' : Addr) (z1 z2 : Z) :
+Lemma phys_addr_add_assoc (a a' : PhysAddr) (z1 z2 : Z) :
   (a + z1)%a = Some a' →
   (a + (z1 + z2))%a = (a' + z2)%a.
 Proof. solve_addr. Qed.
 
-Lemma incr_addr_le (a1 a2 a3 : Addr) (z1 z2 : Z) :
+Lemma incr_phys_addr_le (a1 a2 a3 : PhysAddr) (z1 z2 : Z) :
   (a1 + z1)%a = Some a2 -> (a1 + z2)%a = Some a3 -> (z1 <= z2)%Z ->
   (a2 <= a3)%Z.
 Proof. solve_addr. Qed.
 
-Lemma incr_addr_ne a i :
-  i ≠ 0%Z → a ≠ top →
+Lemma incr_phys_addr_ne (a: PhysAddr) i :
+  i ≠ 0%Z → a ≠ top_phys →
   (a ^+ i)%a ≠ a.
 Proof. intros H1 H2. intro. apply H2. solve_addr. Qed.
 
-Lemma incr_addr_ne_top a z a' :
+Lemma incr_phys_addr_ne_top (a a': PhysAddr) z :
   (z > 0)%Z → (a + z)%a = Some a' →
-  a ≠ top.
+  a ≠ top_phys.
 Proof. intros. intro. solve_addr. Qed.
 
-Lemma get_addrs_from_option_addr_comm a i k :
+Lemma get_phys_addrs_from_option_phys_addr_comm (a: PhysAddr) i k :
   (k >= 0)%Z -> (i >= 0)%Z ->
   (((a ^+ i) ^+ k)%a) =
   ((a ^+ (i + k)%Z)%a).
 Proof. solve_addr. Qed.
 
-Lemma incr_addr_of_z (a a' : Addr) :
+Lemma incr_phys_addr_of_z (a a' : PhysAddr) :
   (a + 1)%a = Some a' →
   (a + 1)%Z = a'.
 Proof. solve_addr. Qed.
 
-Lemma incr_addr_of_z_i (a a' : Addr) i :
+Lemma incr_phys_addr_of_z_i (a a' : PhysAddr) i :
   (a + i)%a = Some a' →
   (a + i)%Z = a'.
 Proof. solve_addr. Qed.
 
-Lemma invert_incr_addr (a1 a2: Addr) (z:Z):
+Lemma invert_incr_phys_addr (a1 a2: PhysAddr) (z:Z):
+      (a1 + z)%a = Some a2 → (a2 + (- z))%a = Some a1.
+Proof. solve_addr. Qed.
+
+
+
+
+(** Virtual Address arithmetic *)
+
+Lemma virt_addr_add_0 (a: VirtAddr): (a + 0)%a = Some a.
+Proof. solve_addr. Qed.
+
+Lemma incr_virt_addr_one_none (a: VirtAddr) :
+  (a + 1)%a = None ->
+  a = top_virt.
+Proof. solve_addr. Qed.
+
+Lemma incr_virt_addr_opt_add_twice (a: VirtAddr) (n m: Z) :
+  (0 <= n)%Z ->
+  (0 <= m)%Z ->
+  ((a ^+ n) ^+ m)%a = (a ^+ (n + m)%Z)%a.
+Proof. solve_addr. Qed.
+
+Lemma incr_virt_addr_opt_add_twice' (a: VirtAddr) (n m: Z) :
+  (0 <= n)%Z ->
+  (0 <= m)%Z ->
+  ((a ^+ n) ^+ m)%a = (a ^+ (n + m)%Z)%a.
+Proof. zify_addr;[]. (* only one goal! *) lia. Qed.
+
+Lemma virt_top_le_eq (a: VirtAddr) : (top_virt <= a)%a → a = top_virt.
+Proof. solve_addr. Qed.
+
+Lemma virt_top_not_le_eq (a: VirtAddr) : ¬ (a < top_virt)%a → a = top_virt.
+Proof. solve_addr. Qed.
+
+Lemma virt_next_lt (a a' : VirtAddr) :
+  (a + 1)%a = Some a' → (a < a')%Z.
+Proof. solve_addr. Qed.
+
+Lemma virt_next_lt_i (a a' : VirtAddr) (i : Z) :
+  (i > 0)%Z →
+  (a + i)%a = Some a' → (a < a')%Z.
+Proof. solve_addr. Qed.
+
+Lemma virt_next_le_i (a a' : VirtAddr) (i : Z) :
+  (i >= 0)%Z →
+  (a + i)%a = Some a' → (a <= a')%Z.
+Proof. solve_addr. Qed.
+
+Lemma virt_next_lt_top (a : VirtAddr) i :
+  (i > 0)%Z →
+  is_Some (a + i)%a → a ≠ top_virt.
+Proof. intros ? [? ?] ?. solve_addr. Qed.
+
+Lemma virt_addr_next_le (a e : VirtAddr) :
+  (a < e)%Z → ∃ a', (a + 1)%a = Some a'.
+Proof. intros. zify_addr; eauto. exfalso. lia. lia. Qed.
+
+Lemma virt_addr_next_lt (a e : VirtAddr) :
+  (a < e)%Z -> ∃ a', (a + 1)%a = Some a'.
+Proof. intros. zify_addr; eauto. exfalso. lia. lia. Qed.
+
+Lemma virt_addr_next_lt_gt_contr (a e a' : VirtAddr) :
+  (a < e)%Z → (a + 1)%a = Some a' → (e < a')%Z → False.
+Proof. solve_addr. Qed.
+
+Lemma virt_addr_next_lt_le (a e a' : VirtAddr) :
+  (a < e)%Z → (a + 1)%a = Some a' → (a' ≤ e)%Z.
+Proof. solve_addr. Qed.
+
+Lemma virt_addr_abs_next (a e a' : VirtAddr) :
+  (a + 1)%a = Some a' → (a < e)%Z → (Z.abs_nat (e - a) - 1) = (Z.abs_nat (e - a')).
+Proof. solve_addr. Qed.
+
+Lemma incr_virt_addr_trans (a1 a2 a3 : VirtAddr) (z1 z2 : Z) :
+  (a1 + z1)%a = Some a2 → (a2 + z2)%a = Some a3 →
+  (a1 + (z1 + z2))%a = Some a3.
+Proof. solve_addr. Qed.
+
+Lemma virt_addr_add_assoc (a a' : VirtAddr) (z1 z2 : Z) :
+  (a + z1)%a = Some a' →
+  (a + (z1 + z2))%a = (a' + z2)%a.
+Proof. solve_addr. Qed.
+
+Lemma incr_virt_addr_le (a1 a2 a3 : VirtAddr) (z1 z2 : Z) :
+  (a1 + z1)%a = Some a2 -> (a1 + z2)%a = Some a3 -> (z1 <= z2)%Z ->
+  (a2 <= a3)%Z.
+Proof. solve_addr. Qed.
+
+Lemma incr_virt_addr_ne (a: VirtAddr) i :
+  i ≠ 0%Z → a ≠ top_virt →
+  (a ^+ i)%a ≠ a.
+Proof. intros H1 H2. intro. apply H2. solve_addr. Qed.
+
+Lemma incr_virt_addr_ne_top (a a': VirtAddr) z :
+  (z > 0)%Z → (a + z)%a = Some a' →
+  a ≠ top_virt.
+Proof. intros. intro. solve_addr. Qed.
+
+Lemma get_virt_addrs_from_option_virt_addr_comm (a: VirtAddr) i k :
+  (k >= 0)%Z -> (i >= 0)%Z ->
+  (((a ^+ i) ^+ k)%a) =
+  ((a ^+ (i + k)%Z)%a).
+Proof. solve_addr. Qed.
+
+Lemma incr_virt_addr_of_z (a a' : VirtAddr) :
+  (a + 1)%a = Some a' →
+  (a + 1)%Z = a'.
+Proof. solve_addr. Qed.
+
+Lemma incr_virt_addr_of_z_i (a a' : VirtAddr) i :
+  (a + i)%a = Some a' →
+  (a + i)%Z = a'.
+Proof. solve_addr. Qed.
+
+Lemma invert_incr_virt_addr (a1 a2: VirtAddr) (z:Z):
       (a1 + z)%a = Some a2 → (a2 + (- z))%a = Some a1.
 Proof. solve_addr. Qed.
